WIP in uncurry proof

theories/L6_PCPS/inline_correct.v
@@ -1,19 +1,15 @@
-Require Import Common.compM Common.Pipeline_utils L6.cps.
-Require Import Coq.ZArith.ZArith Coq.Lists.List Coq.Strings.String Coq.Sets.Ensembles .
-Import ListNotations.
-Require Import identifiers.
-Require Import L6.state L6.freshen L6.cps_util L6.cps_show L6.ctx L6.hoare L6.inline L6.rename
-        L6.Ensembles_util L6.alpha_conv L6.functions L6.logical_relations L6.tactics L6.eval.
+Require Import Coq.ZArith.ZArith Coq.Lists.List Coq.Strings.String Coq.Sets.Ensembles Coq.Classes.Morphisms.
+Require Import compcert.lib.Maps compcert.lib.Coqlib.
+Require Import L6.cps L6.state L6.freshen L6.cps_util L6.cps_show L6.ctx L6.hoare L6.inline L6.rename L6.identifiers
+        L6.Ensembles_util L6.alpha_conv L6.functions L6.logical_relations L6.tactics L6.eval L6.map_util.
+Require Import Common.compM Common.Pipeline_utils Libraries.CpdtTactics Libraries.maps_util.
 Require Import ExtLib.Structures.Monad.
 Require Import ExtLib.Structures.MonadState.
 Require Import ExtLib.Data.Monads.StateMonad.
-Require Coq.Program.Wf.
-Require Import Program.
-(* Require Import Template.monad_utils. *)
 Require Import Coq.Structures.OrdersEx.
-Require Import Common.compM Libraries.CpdtTactics Libraries.maps_util.
 
 Import MonadNotation.
+Import ListNotations.
 Open Scope monad_scope.
 Open Scope ctx_scope.
 Open Scope fun_scope.
@@ -49,7 +45,7 @@ Section Inline_Eq.
       let f' := apply_r sig f in
       let ys' := apply_r_list sig ys in
       let (s' , inl) := update_letApp _ IH f' t ys' s in
-      (match (inl, M.get f' fm, d) with
+      (match (inl, M.get f fm, d) with
        | (true, Some (t, xs, e), S d') =>
          let sig' := set_list (combine xs ys') sig  in            
          e' <- beta_contract _ IH d' e sig' fm s' ;;
@@ -90,7 +86,7 @@ Section Inline_Eq.
       let f' := apply_r sig f in
       let ys' := apply_r_list sig ys in
       let (s', inl) := update_App _ IH f' t ys' s in
-      (match (inl, M.get f' fm, d) with
+      (match (inl, M.get f fm, d) with
        | (true, Some (t, xs, e), S d') =>
          let sig' := set_list (combine xs ys') sig  in
          beta_contract _ IH d' e sig' fm  s'
@@ -143,33 +139,436 @@ Section Inline_correct.
 
   Context (St : Type) (IH : InlineHeuristic St) (cenv : ctor_env) (P1 : PostT) (PG : PostGT).
 
-  Definition fun_map_inv (fm : fun_map) (rho : env) :=
+
+  Variable (HPost_con : post_constr_compat P1 P1)
+           (HPost_proj : post_proj_compat P1 P1)
+           (HPost_fun : post_fun_compat P1 P1)
+           (HPost_case_hd : post_case_compat_hd P1 P1)
+           (HPost_case_tl : post_case_compat_tl P1 P1)
+           (HPost_app : post_app_compat P1 PG)
+           (HPost_letapp : post_letapp_compat cenv P1 P1 PG)
+           (HPost_letapp_OOT : post_letapp_compat_OOT P1 PG)
+           (HPost_OOT : post_OOT P1)
+           (Hpost_base : post_base P1)
+           (HGPost : inclusion P1 PG)
+           (Hpost_zero : forall e rho, post_zero e rho P1).
+
+           (* (HPost_conG : post_constr_compat PG PG) *)
+           (* (HPost_projG : post_proj_compat PG PG) *)
+           (* (HPost_funG : post_fun_compat PG PG) *)
+           (* (HPost_case_hdG : post_case_compat_hd PG PG) *)
+           (* (HPost_case_tlG : post_case_compat_tl PG PG) *)
+           (* (HPost_appG : post_app_compat PG PG) *)
+           (* (HPost_letappG : post_letapp_compat cenv PG PG PG) *)
+           (* (HPost_letapp_OOTG : post_letapp_compat_OOT PG PG) *)
+           (* (HPost_OOTG : post_OOT PG) *)
+           (* (Hpost_baseG : post_base PG) *)
+           (* (Hless_steps_letapp : remove_steps_letapp cenv P1 P1 P1) *)
+           (* (Hless_steps_letapp' : remove_steps_letapp' cenv P1 P1 P1) *)
+           (* (Hless_steps_letapp_OOT : remove_steps_letapp_OOT cenv P1 P1) *)
+           (* (Hless_steps_letapp_OOT' : remove_steps_letapp_OOT' cenv P1 P1) *)
+           (* (Hpost_zero : forall e rho, post_zero e rho P1). *)
+
+  Definition fun_map_fv (fm : fun_map) : Ensemble var :=
+    fun v => exists f ft xs e, fm ! f = Some (ft, xs, e) /\ v \in occurs_free e.
+
+  Definition fun_map_bv (fm : fun_map) : Ensemble var :=
+    fun v => exists f ft xs e, fm ! f = Some (ft, xs, e) /\ v \in bound_var e.
+
+  Definition funs_in_env (rho : env) : Ensemble var :=
+    fun v => exists r B f, rho!v = Some (Vfun r B f).
+
+  Definition occurs_free_in_val (v : val) : Ensemble var :=
+    match v with
+    | Vfun rho B f => occurs_free_fundefs B
+    | _ => Empty_set _
+    end.
+    
+  Definition occurs_free_in_env (rho : env) : Ensemble var :=
+    fun v => exists x r B f, rho!x = Some (Vfun r B f) /\ v \in occurs_free_fundefs B.
+
+  Definition fun_bindings_val (v : val) :=
+    match v with
+    | Vint _
+    | Vconstr _ _ => Empty_set _ 
+    | Vfun rho B _ => name_in_fundefs B :|: funs_in_env rho
+    end.      
+
+  Definition fun_bindings_env (rho : env) : Ensemble var :=
+    fun f => exists x v, rho!x = Some v /\ f \in fun_bindings_val v.
+
+  Lemma fun_bindings_env_set (rho : env) x v :
+    fun_bindings_env (M.set x v rho) \subset fun_bindings_val v :|: fun_bindings_env rho.
+  Proof.
+    intros z Hin. unfold Ensembles.In, fun_bindings_env in *.
+    destructAll. destruct (peq x x0); subst.
+    - rewrite M.gss in H. inv H. now left; eauto.
+    - rewrite M.gso in H; eauto. right. do 2 eexists. split; eauto.
+  Qed.
+  
+  Lemma fun_bindings_env_set_lists (rho rho' : env) xs vs :
+    set_lists xs vs rho = Some rho' ->    
+    fun_bindings_env rho' \subset \bigcup_(v in FromList vs) (fun_bindings_val v) :|: fun_bindings_env rho.
+  Proof.
+    revert rho' vs. induction xs; intros rho' vs Hset; destruct vs; try now inv Hset.
+    - inv Hset. normalize_sets. rewrite big_cup_Empty_set. sets.
+    - normalize_sets. rewrite Union_big_cup.
+      simpl in Hset. destruct (set_lists xs vs rho) eqn:Hset'; inv Hset.
+      eapply Included_trans. eapply fun_bindings_env_set.
+      rewrite big_cup_Singleton. rewrite <- Union_assoc. eapply Included_Union_compat. now sets.
+      eauto.
+  Qed.
+  
+  Lemma fun_bindings_env_get (rho : env) x v :
+    rho ! x = Some v ->
+    fun_bindings_val v \subset fun_bindings_env rho.
+  Proof.
+    intros Hget z Hin. do 2 eexists. split. eassumption. eassumption.
+  Qed.
+
+  Lemma fun_bindings_env_get_list (rho : env) xs vs :
+    get_list xs rho = Some vs ->
+    \bigcup_(v in FromList vs) (fun_bindings_val v) \subset fun_bindings_env rho.
+  Proof.
+    revert vs. induction xs; intros vs Hget.
+    - destruct vs; try now inv Hget. normalize_sets. rewrite big_cup_Empty_set. sets.
+    - simpl in Hget. destruct (rho!a) eqn:Hgeta; try now inv Hget.
+      destruct (get_list xs rho) eqn:Hgetl; try now inv Hget. inv Hget.
+      normalize_sets. rewrite Union_big_cup. rewrite big_cup_Singleton.
+      eapply Union_Included; eauto.
+      eapply fun_bindings_env_get. eassumption.
+  Qed.
+
+  Lemma fun_bindings_env_def_funs (rho rhoc : env) B0 B :
+    fun_bindings_env (def_funs B0 B rhoc rho) \subset name_in_fundefs B0 :|: funs_in_env rhoc :|: fun_bindings_env rho.
+  Proof.
+    revert rho; induction B; intros rho x HIn. simpl in HIn.
+    - eapply fun_bindings_env_set in HIn. simpl in HIn. inv HIn; eauto.
+      eapply IHB. eassumption.
+    - simpl in HIn. now right.
+  Qed.
+
+  Fixpoint fun_map_inv' (k : nat) (S : Ensemble var) (fm : fun_map) (rho : env) : Prop :=
+    forall f ft xs e rhoc B f',
+      f \in S ->
+      fm ! f = Some (ft, xs, e) ->
+      rho ! f = Some (Vfun rhoc B f') ->
+      find_def f B = Some (ft, xs, e) /\ f = f' /\
+      eq_env_P (occurs_free_fundefs B) rho rhoc /\      
+      match k with
+      | 0%nat => True
+      | S k => fun_map_inv' k (occurs_free_fundefs B) fm (def_funs B B rhoc rhoc)
+      end.
+
+  Definition fun_map_inv (k : nat) (S : Ensemble var) (fm : fun_map) (rho : env) : Prop :=
+    forall f ft xs e rhoc B f',
+      f \in S ->
+      fm ! f = Some (ft, xs, e) ->
+      rho ! f = Some (Vfun rhoc B f') ->
+      find_def f B = Some (ft, xs, e) /\ f = f' /\
+      eq_env_P (occurs_free_fundefs B) rho rhoc /\      
+      match k with
+      | 0%nat => True
+      | S k => fun_map_inv' k (occurs_free_fundefs B) fm (def_funs B B rhoc rhoc)
+      end.
+    
+  Lemma fun_map_inv_eq k fm rho :
+    fun_map_inv k fm rho = fun_map_inv' k fm rho.
+  Proof.
+    destruct k; reflexivity.
+  Qed.
+  
+  Lemma fun_map_inv_mon k k' S fm rho :
+    fun_map_inv k S fm rho ->
+    (k' <= k)%nat ->
+    fun_map_inv k' S fm rho.
+  Proof.
+    revert S k fm rho. induction k' as [k' IHk] using lt_wf_rec1; intros.
+    destruct k'.
+    - unfold fun_map_inv in *. intros. edestruct H as [Hf [Heq [Heq' Hm]]]; eauto. 
+    - destruct k; [ omega | ].
+      intro; intros. edestruct H as [Hf [Heq [Heq' Hm]]]; eauto. 
+      split; eauto. split; eauto. split; eauto. rewrite <- fun_map_inv_eq. eapply IHk. 
+      omega. rewrite fun_map_inv_eq. eassumption. omega. 
+  Qed.
+  
+  Lemma fun_map_inv_set k S fm rho x v :
+    fun_map_inv k S fm rho ->
+    ~ x \in Dom_map fm :|: occurs_free_in_env rho  ->
+    fun_map_inv k (x |: S) fm (M.set x v rho).           
+  Proof.
+    intros Hinv Hnin. intro; intros.
+    rewrite M.gso in *.
+    2:{ intros Heq; subst. eapply Hnin. left. eexists; eauto. }
+    inv H.
+    - inv H2. exfalso. eapply Hnin. left. eexists; eauto.
+    - edestruct Hinv; eauto.
+      destructAll. split; [| split; [| split ]]; eauto.
+      eapply eq_env_P_set_not_in_P_l. eassumption.
+      intros Hc. eapply Hnin. right. do 4 eexists. split; eauto.    
+  Qed.
+
+  (* Lemma occurs_free_in_env_set_compat rho rho' x v : *)
+  (*   occurs_free_in_env rho' \subset occurs_free_in_env rho -> *)
+  (*   occurs_free_in_env (M.set x v rho') \subset occurs_free_in_env (M.set x v rho). *)
+  (* Proof. *)
+  (*   intros Hc z [y Hin]. destructAll. *)
+  (*   destruct (peq x y); subst. *)
+  (*   - rewrite M.gss in H. inv H.  *)
+  (*     do 4 eexists; split; eauto. rewrite M.gss. reflexivity. *)
+  (*   - rewrite M.gso in H; eauto. edestruct Hc. now do 4 eexists; split; eauto. *)
+  (*     destructAll. do 4 eexists; split; eauto. rewrite M.gso. eassumption. reflexivity. *)
+  (*   rewrite M.gso. eassumption. *)
+  (*   intros Hd. eapply Hc. subst. eexists. eassumption. *)
+  (* Qed. *)
+      
+  Lemma occurs_free_in_env_set rho x v :
+    occurs_free_in_env (M.set x v rho) \subset occurs_free_in_val v :|: occurs_free_in_env rho.
+  Proof.
+    intros z [y Hin]. destructAll. destruct (peq x y); subst.
+    - rewrite M.gss in H. inv H. now left; eauto.
+    - rewrite M.gso in H; eauto. right.
+      do 4 eexists; split; eauto.
+  Qed.
+
+  Lemma occurs_free_in_env_set_lists_not_In rho rho' xs vs :
+    set_lists xs vs rho = Some rho' ->
+    occurs_free_in_env rho' \subset \bigcup_(v in FromList vs) (occurs_free_in_val v) :|: occurs_free_in_env rho.
+  Proof.
+    revert rho' vs. induction xs; intros rho' vs Hset; destruct vs; try now inv Hset.
+    - inv Hset. normalize_sets. rewrite big_cup_Empty_set. sets.
+    - normalize_sets. rewrite Union_big_cup.
+      simpl in Hset. destruct (set_lists xs vs rho) eqn:Hset'; inv Hset.
+      eapply Included_trans. eapply occurs_free_in_env_set.
+      rewrite big_cup_Singleton. rewrite <- Union_assoc. eapply Included_Union_compat. now sets.
+      eauto.
+  Qed.
+
+  Instance fm_map_Proper k : Proper (Same_set _ ==> eq ==> eq ==> iff) (fun_map_inv k).
+  Proof.
+    repeat (intro; intros). subst. split; intros.
+    intro; intros. rewrite <- H in H1. eauto.
+    intro; intros. rewrite H in H1. eauto.
+  Qed.
+  
+  Lemma fun_map_inv_set_lists k S fm rho rho' xs vs :
+    fun_map_inv k S fm rho ->
+    \bigcup_(v in FromList vs) (occurs_free_in_val v) \subset occurs_free_in_env rho ->
+    Disjoint _ (FromList xs) (Dom_map fm :|: occurs_free_in_env rho) ->
+    set_lists xs vs rho = Some rho' ->
+    fun_map_inv k (FromList xs :|: S) fm rho'.
+  Proof.
+    revert S rho rho' vs; induction xs; intros S rho rho' vs Hfm Hs Hdis Hset.
+    - destruct vs; inv Hset; eauto. repeat normalize_sets. eauto.
+    - destruct vs; try now inv Hset. simpl in Hset.
+      destruct (set_lists xs vs rho) eqn:Hset'; inv Hset.
+      repeat normalize_sets. rewrite <- Union_assoc. eapply fun_map_inv_set.
+      eapply IHxs; eauto.
+      + eapply Included_trans; [| eassumption ]. eapply Included_big_cup. reflexivity.
+        sets.
+      + sets.
+      + intros Hc. eapply Hdis. constructor. now left. inv Hc; eauto.
+        eapply occurs_free_in_env_set_lists_not_In in H; [| now eauto ]. inv H; eauto.
+        right. eapply Hs. eapply Included_big_cup; [| | eassumption ]. reflexivity. sets.
+  Qed.
+  
+  Lemma add_fundefs_in fm f B ft xs e:
+    find_def f B = Some (ft, xs, e) -> 
+    (add_fundefs B fm) ! f = Some (ft, xs, e). 
+  Proof.
+    induction B.
+    - simpl. intros Hdef. destruct (M.elt_eq f v); subst.
+      + inv Hdef. simpl. rewrite M.gss. reflexivity.
+      + simpl. rewrite M.gso; eauto.
+    - intros H. inv H.
+  Qed.
+
+  Lemma add_fundefs_not_in fm f B :
+    ~ f \in name_in_fundefs B -> 
+    (add_fundefs B fm) ! f = fm ! f.
+  Proof.
+    intros Hnin. induction B.
+    - simpl. rewrite M.gso. eapply IHB.
+      intros Hc. eapply Hnin. simpl. now right; eauto.
+      intros Hc. eapply Hnin. simpl. subst; eauto.
+    - reflexivity.
+  Qed.
+
+  Lemma Dom_map_add_fundefs fm B :
+    Dom_map (add_fundefs B fm) <--> name_in_fundefs B :|: Dom_map fm.
+  Proof.
+    induction B; simpl; [| now sets ].
+    rewrite Dom_map_set. rewrite IHB. sets.
+  Qed.
+
+  Lemma fun_map_inv_def_funs k fm rho B :
+    fun_map_inv k fm rho ->
+    Disjoint _ (name_in_fundefs B) (fun_bindings_env rho) ->
+    fun_map_inv k (add_fundefs B fm) (def_funs B B rho rho).
+  Proof.
+    revert fm rho B. induction k as [k IHk] using lt_wf_rec1. intros fm rho B Hf Hdis.
+    intros f ft xs e rhoc B' f' Heq1 Heq2.  
+    destruct (Decidable_name_in_fundefs B) as [Dec]. destruct (Dec f).
+    - rewrite def_funs_eq in Heq2; eauto. inv Heq2.
+      edestruct name_in_fundefs_find_def_is_Some. eassumption. destructAll.
+      erewrite add_fundefs_in in Heq1; [| eassumption ]. inv Heq1. split; eauto.
+      split; eauto. destruct k; eauto. rewrite <- fun_map_inv_eq. eapply IHk. omega.
+      eapply fun_map_inv_mon. eassumption. omega.
+      eassumption.
+    - rewrite def_funs_neq in Heq2; eauto.
+      rewrite add_fundefs_not_in in Heq1; [| eassumption ].
+      edestruct Hf. eassumption. eassumption. destructAll. split; eauto. split; eauto. 
+      destruct k; eauto. rewrite <- fun_map_inv_eq in *.
+      assert (Hdis' : Disjoint _ (name_in_fundefs B) (name_in_fundefs B' :|: funs_in_env rhoc)).
+      { eapply Disjoint_Included_r; [| eassumption ].
+        eapply Included_trans; [| eapply fun_bindings_env_get ]; [| eassumption ].
+        reflexivity. }      
+      clear Dec H Hf Heq2 Hdis. 
+      revert rhoc B' B n H1 Hdis'. induction k as [k IHk2] using lt_wf_rec1; intros.
+      intro; intros.
+      rewrite add_fundefs_not_in in H; eauto. 
+      edestruct H1. eassumption. eassumption. destructAll. split; eauto. split; eauto.
+      destruct k; eauto. rewrite <- fun_map_inv_eq in *. 
+      eapply IHk2. omega. now eauto. eassumption. eassumption. admit. eassumption. 
+      { intros Hc.
+        eapply Hdis. constructor. eassumption. SearchAbout rho.
+        destruct (Decidable_name_in_fundefs B') as [Dec]. destruct (Dec f).
+        
+
+        intros Hin. eapply Hdis. constructor. eassumption. eapply H1. eassumption.
+  Qed.
+
+(*   
+  Definition fun_map_inv (fm : fun_map) (rho : env) (* (sig : subst) *) :=
     forall f ft xs e,
       fm ! f = Some (ft, xs, e) ->
-      exists rhoc B g, rho ! f = Some (Vfun rhoc B g) /\
-                       find_def g B = Some (ft, xs, e).
-
+      exists rhoc B, rho ! f = Some (Vfun rhoc B f) /\
+                     find_def f B = Some (ft, xs, e) /\
+                     (forall g, g \in name_in_fundefs B ->
+                                rho ! g = Some (Vfun rhoc B g) /\ g \in Dom_map fm).
   
   Lemma fun_map_inv_set fm rho x v :
     fun_map_inv fm rho ->
     ~ x \in Dom_map fm ->
     fun_map_inv fm (M.set x v rho).           
-
-  Lemma fun_map_inv_set_lists fm rho xs vs :
+  Proof.
+    intros Hinv Hnin f ft xs e Hget.
+    rewrite M.gso.
+    - eapply Hinv in Hget. destructAll. do 2 eexists. split; eauto. split; eauto.
+      intros. rewrite M.gso. eauto. intro; subst. eapply H1 in H2.
+      inv H2. contradiction.
+    - intros Heq; subst. eapply Hnin.
+      eexists; eauto.
+  Qed.
+    
+  Lemma fun_map_inv_set_lists fm rho rho' xs vs :
     fun_map_inv fm rho ->
     Disjoint _ (FromList xs) (Dom_map fm) ->
     set_lists xs vs rho = Some rho' ->
     fun_map_inv fm rho'.
+  Proof.
+    revert rho rho' vs; induction xs; intros rho rho' vs Hfm Hdis Hset.
+    - destruct vs; inv Hset; eauto.
+    - destruct vs; try now inv Hset. simpl in Hset.
+      destruct (set_lists xs vs rho) eqn:Hset'; inv Hset.
+      repeat normalize_sets.
+      eapply fun_map_inv_set. eapply IHxs; eauto.
+      now sets. intros Hc. eapply Hdis. constructor. now left.
+      eassumption.
+  Qed.
+  
+  Lemma add_fundefs_in fm f B ft xs e:
+    find_def f B = Some (ft, xs, e) -> 
+    (add_fundefs B fm) ! f = Some (ft, xs, e). 
+  Proof.
+    induction B.
+    - simpl. intros Hdef. destruct (M.elt_eq f v); subst.
+      + inv Hdef. simpl. rewrite M.gss. reflexivity.
+      + simpl. rewrite M.gso; eauto.
+    - intros H. inv H.
+  Qed.
+
+  Lemma add_fundefs_not_in fm f B :
+    ~ f \in name_in_fundefs B -> 
+    (add_fundefs B fm) ! f = fm ! f.
+  Proof.
+    intros Hnin. induction B.
+    - simpl. rewrite M.gso. eapply IHB.
+      intros Hc. eapply Hnin. simpl. now right; eauto.
+      intros Hc. eapply Hnin. simpl. subst; eauto.
+    - reflexivity.
+  Qed.
+
+  Lemma Dom_map_add_fundefs fm B :
+    Dom_map (add_fundefs B fm) <--> name_in_fundefs B :|: Dom_map fm.
+  Proof.
+    induction B; simpl; [| now sets ].
+    rewrite Dom_map_set. rewrite IHB. sets.
+  Qed.
 
   Lemma fun_map_inv_def_funs fm rho B :
-    fun_map_inv fm rho -
+    fun_map_inv fm rho ->
+    Disjoint _ (name_in_fundefs B) (Dom_map fm) ->
     fun_map_inv (add_fundefs B fm) (def_funs B B rho rho).
-    
+  Proof.
+    intros Hf Hd. intros f ft xs e Hget.
+    destruct (Decidable_name_in_fundefs B) as [Dec]. destruct (Dec f).
+    - do 2 eexists. split; [| split; [| split ]].
+      + eapply def_funs_eq in n. eassumption.
+      + edestruct name_in_fundefs_find_def_is_Some. eassumption.
+        destructAll. rewrite H. eapply add_fundefs_in in H. rewrite H in Hget.
+        inv Hget. reflexivity.
+      + rewrite def_funs_eq. reflexivity. eassumption.
+      + rewrite Dom_map_add_fundefs. sets.
+    - rewrite add_fundefs_not_in in Hget; [| eassumption ]. rewrite def_funs_neq; eauto.
+      eapply Hf in Hget. destructAll. do 2 eexists. split; eauto. split; eauto.
+      intros. rewrite def_funs_neq; eauto. split; eauto. eapply H1. eassumption.
+      rewrite Dom_map_add_fundefs. right. eapply H1; eauto.
+      intros Hin. eapply Hd. constructor. eassumption. eapply H1. eassumption.
+  Qed.
+*)
+  (* Lemma fun_map_inv_redef_funs fm rho B ft xs e rhoc f  : *)
+  (*   fun_map_inv fm rho -> *)
+  (*   fm ! f = Some (ft, xs, e) -> *)
+  (*   rho ! f = Some (Vfun rhoc B f) -> *)
+  (*   fun_map_inv fm (def_funs B B rho rho). *)
+  (* Proof. *)
+  (*   intros Hf Hg1 Hg2. intros g ft' xs' e' Hget. *)
+  (*   destruct (Decidable_name_in_fundefs B) as [Dec]. destruct (Dec g). *)
+  (*   - assert (Hg1' := Hg1). eapply Hf in Hg1. destructAll.  *)
+  (*     rewrite Hg2 in H. inv H. erewrite def_funs_eq; eauto. *)
+  (*     do 2 eexists. split. reflexivity. *)
+  (*     eapply H1 in n. destructAll. destruct H2. destruct x1 as [[? ? ] ?]. rewrite Hget in H2; inv H2.  *)
+  (*     eapply Hf in Hget. destructAll. rewrite H2 in H. inv H. split. eassumption. *)
+  (*     intros. rewrite def_funs_eq; eauto. split. reflexivity. eapply H4. eassumption. *)
+  (*   - rewrite def_funs_neq; eauto. *)
+  (*     eapply Hf in Hget. destructAll. do 2 eexists. split; eauto. split; eauto. *)
+
+  (*     intros g1 Hc. destruct (Decidable_name_in_fundefs B) as [Dec']. destruct (Dec' g1). clear Dec Dec'. *)
+  (*     + eapply Hf in Hg1. destructAll. repeat subst_exp.  *)
+  (*       eapply H4 in n0. destructAll.  *)
+  (*       eapply H1 in Hc. destructAll. repeat subst_exp.  *)
+  (*       rewrite def_funs_eq; eauto. *)
+        
+  (*       split. reflexivity. *)
+  (*     repeat subst_exp. do 10 subst_exp.  *)
+      (*   destruct (Decidable_name_in_fundefs B) as [Dec]. destruct (Dec f). *)
+  (*   - do 3 eexists. split. *)
+  (*     + eapply def_funs_eq in n. eassumption. *)
+  (*     + edestruct name_in_fundefs_find_def_is_Some. eassumption. *)
+  (*       destructAll. rewrite H. eapply add_fundefs_in in H. rewrite H in Hget. *)
+  (*       inv Hget. reflexivity. *)
+  (*   - rewrite add_fundefs_not_in in Hget; [| eassumption ]. rewrite def_funs_neq; eauto. *)
+  (* Qed. *)
+  (* Abort. *)
+  
+  Opaque preord_exp'.
+  
   Lemma inline_correct d e sig fm st S :
     unique_bindings e ->
     Disjoint _ (bound_var e) (occurs_free e) ->
     Disjoint _ S (bound_var e :|: image (apply_r sig) (occurs_free e)) ->
-    Disjoint _ (Dom_map fm) (bound_var e) ->
+    Disjoint _ (Dom_map fm) (bound_var e) ->       
     {{ fun _ s => fresh S (next_var (fst s)) }}
       beta_contract St IH d e sig fm st
     {{ fun _ _ e' s' =>
@@ -184,12 +583,13 @@ Section Inline_correct.
          (* semantics are preserved *)
          (forall rho1 rho2 k,
              preord_env_P_inj cenv PG (occurs_free e) k (apply_r sig) rho1 rho2 ->
+             fun_map_inv fm rho1 ->
              preord_exp cenv P1 PG k (e, rho1) (e', rho2))
 
     }}.
   Proof.
     revert e sig fm st S. induction d as [d IHd] using lt_wf_rec1.
-    induction e using exp_ind'; intros sig fm st S Hun Hdis1 Hdis2; inv Hun; rewrite beta_contract_eq.
+    induction e using exp_ind'; intros sig fm st S Hun Hdis1 Hdis2 Hdis3; inv Hun; rewrite beta_contract_eq.
     - (* constr *)
       eapply bind_triple. now eapply get_name_fresh. 
       intros x w1. eapply pre_curry_l. intros Hinx.
@@ -207,6 +607,7 @@ Section Inline_correct.
         eapply Union_Disjoint_r. now sets.
         eapply Disjoint_Included; [| | eapply Hdis2 ]. rewrite image_Union. now sets.
         now sets.
+      + repeat normalize_bound_var_in_ctx. sets.
       + intros e' w2. eapply return_triple.
         intros _ st'. intros [Hf [Hun [Hsub [Hsub' Hsem]]]].
         split; [| split; [| split; [| split ]]].
@@ -220,17 +621,69 @@ Section Inline_correct.
           rewrite Setminus_Union_distr. rewrite Setminus_Same_set_Empty_set. normalize_sets. sets.
         * normalize_bound_var. eapply Union_Included. eapply Included_trans. eassumption. now sets.
           eapply Singleton_Included. eassumption.
-        * intros r1 r2 k Henv. eapply preord_exp_const_compat.
+        * intros r1 r2 k Henv Hfm. eapply preord_exp_const_compat.
           admit. admit. admit.
           intros. eapply Hsem. 
           rewrite apply_r_set_f_eq. eapply preord_env_P_inj_set_alt.
           -- eapply preord_env_P_inj_antimon. eapply preord_env_P_inj_monotonic; [| eassumption ].
              omega. normalize_occurs_free. sets.
           -- rewrite preord_val_eq. split. reflexivity.
-             eapply Forall2_Forall2_asym_included. eassumption. 
+             eapply Forall2_Forall2_asym_included. eassumption.
           -- intros Hc. eapply Hdis2. constructor. eassumption.
              right. normalize_occurs_free. rewrite image_Union. right. eassumption.
-    - 
+          -- eapply fun_map_inv_set. eassumption.
+             eapply Disjoint_Singleton_In. tci. repeat normalize_bound_var_in_ctx. sets.
+    - (* Ecase [] *)
+      admit.
+    - (* Ecase (_ :: _) *)
+      admit.
+    - (* Eproj *)
+      admit.
+    - (* Eletapp *)
+      admit.
+    - (* Efun *)
+      admit.
+    - (* Eapp *)
+      simpl. destruct (update_App St IH (apply_r sig v) t (apply_r_list sig l) st) as [s b] eqn:Hup. 
+      + destruct b.
+        * destruct (fm ! v) as [[[ft xs] e] |] eqn:Heqf.
+          destruct d.
+          -- eapply return_triple.
+             intros. split; [| split; [| split; [| split ]]]; try eassumption.
+             ++ constructor.
+             ++ simpl. repeat normalize_occurs_free. rewrite image_Union, image_Singleton.
+                rewrite FromList_apply_list. reflexivity.
+             ++ normalize_bound_var. sets.
+             ++ intros. eapply preord_exp_app_compat.
+                assumption. assumption.
+                eapply H0. now constructor.
+                eapply Forall2_preord_var_env_map. eassumption.
+                now constructor.
+          -- eapply post_weakening; [| eapply IHd ].
+             ++ simpl. intros. destructAll. 
+                split; [| split; [| split; [| split ]]]; try eassumption.
+                ** eapply Included_trans. eassumption.
+                   (* eapply Included_trans. eapply image_apply_r_set_list.  eassumption.  *)
+                   admit. (* change FV subset to include fvs in fm *)
+                ** intros. eapply preord_exp_app_l.
+                   --- admit.
+                   --- admit. 
+                   --- intros. assert (Heqf' := Heqf). eapply H6 in Heqf. destructAll.
+                       do 2 subst_exp. eapply H4.
+                       admit. 
+                       eapply fun_map_inv_set_lists.
+                       eapply  fun_map_inv_def_funs.
+                       eassumption.
+                       admit.
+                       (* eapply Disjoint_sym. eapply Disjoint_Included_r; [| eassumption ]. *)
+                       
+                       normalize_bound_var. 
+                       H4. 
+                normalize_occurs_free; sets.
+             split.
+             
+      simpl. 
+       eapply bind_triple.
           pre
           reflexivity. 
         rewrite Union_Setminus with (S1 := occurs_free e) (S2 := [set v]).
